theories/Template/QuoteGround/Init/Typing.v
@@ -1,0 +1,78 @@
+From MetaCoq.Template Require Import MonadBasicAst MonadAst All utils.
+From MetaCoq.Template Require Import Typing utils.bytestring TermEquality ReflectAst Ast Reflect.
+From MetaCoq.Lob.Template Require Export QuoteGround.Init.
+Export utils.bytestring.
+Require Import Coq.Lists.List.
+Import ListNotations.
+
+Local Set Primitive Projections.
+Local Open Scope bs.
+Import MCMonadNotation.
+
+Module config.
+  Class typing_restriction
+    := { checker_flags_constraint : config.checker_flags -> bool
+       ; global_env_ext_constraint : global_env_ext -> bool }.
+End config.
+
+Class quotation_of_well_typed {Pcf : config.typing_restriction} {T} (t : T) {qT : quotation_of T} {qt : quotation_of t} := typing_quoted_term_of : forall cf Σ Γ, config.checker_flags_constraint cf -> config.global_env_ext_constraint Σ -> wf_local Σ Γ -> Σ ;;; Γ |- qt : qT.
+Class ground_quotable_well_typed {Pcf : config.typing_restriction} T {qT : quotation_of T} {quoteT : ground_quotable T} := typing_quote_ground : forall t : T, quotation_of_well_typed t.
+
+Inductive dynlist := dnil | dcons {T} (t : T) (tl : dynlist).
+Declare Scope dynlist_scope.
+Delimit Scope dynlist_scope with dynlist.
+Bind Scope dynlist_scope with dynlist.
+Infix "::" := dcons : dynlist_scope.
+Notation "[ ]" := dnil : dynlist_scope.
+Notation "[ x ]" := (dcons x dnil) : dynlist_scope.
+Notation "[ x ; y ; .. ; z ]" :=  (dcons x (dcons y .. (dcons z dnil) ..)) : dynlist_scope.
+
+Fixpoint quote_dynlist (d : dynlist) : TemplateMonad (list term)
+  := match d with
+     | dnil => ret []
+     | dcons _ t rest => qt <- tmQuote t;; qts <- quote_dynlist rest;; ret (qt :: qts)
+     end.
+
+Definition constraint_for_globals (globals : dynlist) : TemplateMonad (global_env_ext -> bool)
+  := qts <- quote_dynlist globals;;
+     inds <- monad_map (fun qt => match qt with
+                                  | tInd {| inductive_mind := mind |} _
+                                    => ind <- tmQuoteInductive mind;;
+                                       (*tmPrint ind;;*)
+                                       ret (mind, ind)
+                                  | _ => tmPrint ("ensure present not inductive"%bs, qt);; tmFail "ensure present not inductive"%bs
+                                  end) qts;;
+     ret (fun Σ : global_env_ext
+          => List.fold_right andb true (List.map (fun '(mind, ind) => lookup_env Σ.1 mind == Some (InductiveDecl ind)) inds)).
+
+Notation ground_quotable_well_typed_using ls T
+  := (match ls%dynlist, T return _ with
+      | globals, T'
+        => ltac:(let T' := (eval cbv delta [T'] in T') in
+                 run_template_program
+                   (constraint_for_globals globals)
+                   (fun c => refine (@ground_quotable_well_typed
+                                       {| config.checker_flags_constraint := _.(config.checker_flags_constraint)
+                                       ; config.global_env_ext_constraint := c |}
+                                       T' _ _)))
+      end)
+       (only parsing).
+Notation quotation_of_well_typed_using ls t
+  := (match ls%dynlist, t return _ with
+      | globals, t'
+        => ltac:(let t' := (eval cbv delta [t'] in t') in
+                 run_template_program
+                   (constraint_for_globals globals)
+                   (fun c => refine (@quotation_of_well_typed
+                                       {| config.checker_flags_constraint := _.(config.checker_flags_constraint)
+                                       ; config.global_env_ext_constraint := c |}
+                                       _ t' _ _)))
+      end)
+       (only parsing).
+
+Module Export Instances.
+  #[export] Instance default_typing_restriction : config.typing_restriction | 1000
+    := {| config.checker_flags_constraint cf := true
+       ; config.global_env_ext_constraint Σ := true |}.
+  #[export] Existing Instance typing_quote_ground.
+End Instances.
